src/FlatCompCombined.v
@@ -1,0 +1,93 @@
+Require Import compcert.driver.Compiler compcert.common.Errors.
+Require Import Common Monads.
+Require CompilationUnit.
+Require Import Metadata.
+
+Require LocalsOnly FlatIntTag.
+Require
+    FlatSwitchComp
+    FlatSeqComp
+    FlatSeqComp2
+    FlatSeqStmtComp
+    FlatReturnComp
+    FlatExprComp
+    FlatExprRetComp
+    FlatStopComp
+    FlatDestCheckComp
+    FlatIntTagComp
+.
+
+Definition option_to_res {A} (o : option A) : res A :=
+  match o with
+  | None => Error []
+  | Some a => OK a
+  end.
+Coercion option_to_res : option >-> res.
+
+Definition compile_cu (cu : LocalsOnly.env * list metadata) :
+        res (FlatIntTag.env * list metadata) :=
+  OK cu
+  @@ FlatSwitchComp.compile_cu
+  @@ FlatSeqComp.compile_cu
+  @@ FlatSeqComp2.compile_cu
+  @@ FlatSeqStmtComp.compile_cu
+  @@ FlatReturnComp.compile_cu
+  @@ FlatExprComp.compile_cu
+  @@ FlatExprRetComp.compile_cu
+  @@ FlatStopComp.compile_cu
+  @@ FlatDestCheckComp.compile_cu
+ @@@ FlatIntTagComp.compile_cu.
+
+Inductive I : LocalsOnly.state -> FlatIntTag.state -> Prop :=
+| ICombined : forall s00 s01 s02 s03 s04 s05 s06 s07 s08 s09 s10,
+        FlatSwitchComp.I    s00 s01 ->
+        FlatSeqComp.I       s01 s02 ->
+        FlatSeqComp2.I      s02 s03 ->
+        FlatSeqStmtComp.I   s03 s04 ->
+        FlatReturnComp.I    s04 s05 ->
+        FlatExprComp.I      s05 s06 ->
+        FlatExprRetComp.I   s06 s07 ->
+        FlatStopComp.I      s07 s08 ->
+        FlatDestCheckComp.I s08 s09 ->
+        FlatIntTagComp.I    s09 s10 ->
+        I s00 s10.
+
+Inductive I_func : list LocalsOnly.insn * nat -> FlatIntTag.stmt * FlatIntTag.expr -> Prop :=
+| IFuncCombined : forall f00 f01 f02 f03 f04 f05 f06 f07 f08 f09 f10,
+        FlatSwitchComp.I_func       f00 f01 ->
+        FlatSeqComp.I_func          f01 f02 ->
+        FlatSeqComp2.I_func         f02 f03 ->
+        FlatSeqStmtComp.I_func      f03 f04 ->
+        FlatReturnComp.I_func       f04 f05 ->
+        FlatExprComp.I_func         f05 f06 ->
+        FlatExprRetComp.I_func      f06 f07 ->
+        FlatStopComp.I_func         f07 f08 ->
+        FlatDestCheckComp.I_func    f08 f09 ->
+        FlatIntTagComp.I_func       f09 f10 ->
+        I_func f00 f10.
+
+Lemma chain_I_env :
+    forall e00 e01 e02 e03 e04 e05 e06 e07 e08 e09 e10,
+        Forall2 FlatSwitchComp.I_func       e00 e01 ->
+        Forall2 FlatSeqComp.I_func          e01 e02 ->
+        Forall2 FlatSeqComp2.I_func         e02 e03 ->
+        Forall2 FlatSeqStmtComp.I_func      e03 e04 ->
+        Forall2 FlatReturnComp.I_func       e04 e05 ->
+        Forall2 FlatExprComp.I_func         e05 e06 ->
+        Forall2 FlatExprRetComp.I_func      e06 e07 ->
+        Forall2 FlatStopComp.I_func         e07 e08 ->
+        Forall2 FlatDestCheckComp.I_func    e08 e09 ->
+        Forall2 FlatIntTagComp.I_func       e09 e10 ->
+        Forall2 I_func e00 e10.
+intros.
+list_magic_on (e00, (e01, (e02, (e03, (e04, (e05, (e06, (e07, (e08, (e09, (e10, tt))))))))))).
+eapply IFuncCombined; eassumption.
+Qed.
+
+Theorem compile_I_func : forall a ameta b bmeta,
+    compile_cu (a, ameta) = Some (b, bmeta) ->
+    Forall2 I_func a b.
+intros0 Hcomp. unfold compile_cu in *.
+match goal with
+| [ H : context [ ?l @@ ?r ] |- _ ] => idtac l; idtac r
+end.
